src/Pipit.System.Exp.Check.Contracts.fst
@@ -1,0 +1,243 @@
+(* Properties about contract definitions *)
+module Pipit.System.Exp.Check.Contracts
+
+open Pipit.Prim.Table
+open Pipit.Exp.Base
+open Pipit.System.Exp.Check.Base
+
+module SXCA = Pipit.System.Exp.Check.Assumptions
+module SXCO = Pipit.System.Exp.Check.Obligations
+module SXCI = Pipit.System.Exp.Check.Invariants
+
+module CR  = Pipit.Context.Row
+
+module SB  = Pipit.System.Base
+module SX  = Pipit.System.Exp
+module SXP = Pipit.System.Exp.Properties
+module SI  = Pipit.System.Ind
+
+module XB  = Pipit.Exp.Bigstep
+module XC  = Pipit.Exp.Causality
+module XK  = Pipit.Exp.Checked.Base
+
+module PM = Pipit.Prop.Metadata
+
+module List = FStar.List.Tot
+module T    = FStar.Tactics
+
+#push-options "--split_queries always"
+
+let rec contract_invariant_holds
+  (#t: table) (#c: context t) (#a: t.ty)
+  (rows: list (row c) { Cons? rows })
+  (r: exp t       c  t.propty { XC.causal r })
+  (g: exp t (a :: c) t.propty { XC.causal g })
+  (b: exp t       c         a { XC.causal b }):
+  Lemma
+    (ensures (
+      let vs  = XC.lemma_bigsteps_total_vs rows b in
+      let rows'=CR.extend1 vs rows in
+      let t   = SX.system_of_contract r g b in
+      let ios = inputs_with_oracles_contract_definition rows r g b in
+      let stp = SI.system_step_result t ios in
+
+      let iosr = inputs_with_oracles rows r in
+      let stpr = SI.system_step_result (SX.system_of_exp r) iosr in
+
+      let iosg = inputs_with_oracles rows' g in
+      let stpg = SI.system_step_result (SX.system_of_exp g) iosg in
+
+      let iosb = inputs_with_oracles rows b in
+      let stpb = SI.system_step_result (SX.system_of_exp b) iosb in
+
+      SXP.system_of_contract_invariant rows r g b stp.s /\
+      stp.s == SB.type_join_tup stpr.s (SB.type_join_tup stpg.s stpb.s) /\
+      (SB.option_prop_sem stp.chck.assumptions <==> (
+        b2t stpr.v /\
+        SB.option_prop_sem stpr.chck.assumptions /\
+        SB.option_prop_sem stpg.chck.assumptions /\
+        SB.option_prop_sem stpb.chck.assumptions)) /\
+      (SB.option_prop_sem stp.chck.obligations <==> (
+        b2t stpg.v /\
+        SB.option_prop_sem stpr.chck.obligations /\
+        SB.option_prop_sem stpg.chck.obligations /\
+        SB.option_prop_sem stpb.chck.obligations)) /\
+      (stpr.v == XC.lemma_bigstep_total_v rows r) /\
+      (stpg.v == XC.lemma_bigstep_total_v rows' g) /\
+      (stpb.v == XC.lemma_bigstep_total_v rows b) /\
+      (stp.v  == XC.lemma_bigstep_total_v rows b)
+    ))
+  =
+  let vs  = XC.lemma_bigsteps_total_vs rows b in
+  let rows'=CR.extend1 vs rows in
+  let t   = SX.system_of_contract r g b in
+  let ios = inputs_with_oracles_contract_definition rows r g b in
+  let stp = SI.system_step_result t ios in
+
+  let iosr = inputs_with_oracles rows r in
+  let stpr = SI.system_step_result (SX.system_of_exp r) iosr in
+
+  let iosg = inputs_with_oracles rows' g in
+  let stpg = SI.system_step_result (SX.system_of_exp g) iosg in
+
+  let iosb = inputs_with_oracles rows b in
+  let stpb = SI.system_step_result (SX.system_of_exp b) iosb in
+
+  let o = SB.type_join_tup
+    (SXP.step_oracle rows r)
+    (SB.type_join_tup
+      (SXP.step_oracle rows' g)
+      (SXP.step_oracle rows b))
+  in
+  match rows with
+  | [row1] ->
+    SXP.invariant_init r;
+    SXP.invariant_init g;
+    SXP.invariant_init b;
+
+    SXP.invariant_step [] row1  r (SX.system_of_exp r).init;
+    SXP.invariant_step [] (CR.cons stp.v row1) g (SX.system_of_exp g).init;
+    SXP.invariant_step [] row1 b (SX.system_of_exp b).init;
+
+    assert (vs == [stpb.v]);
+    assert (rows' == [stpb.v, row1]);
+    assert (stp == t.step (List.hd rows) o t.init);
+    assert (stpr == (SX.system_of_exp r).step (List.hd rows) (SB.type_join_fst o) (SB.type_join_fst t.init));
+    assert (stpb == (SX.system_of_exp b).step (List.hd rows) (SB.type_join_snd (SB.type_join_snd o)) (SB.type_join_snd (SB.type_join_snd t.init)));
+    assert (stpg == (SX.system_of_exp g).step (stpb.v, List.hd rows) (SB.type_join_fst (SB.type_join_snd o)) (SB.type_join_fst (SB.type_join_snd t.init)));
+
+    assert (SB.option_prop_sem stp.chck.assumptions <==> (
+        b2t stpr.v /\
+        SB.option_prop_sem stpr.chck.assumptions /\
+        SB.option_prop_sem stpg.chck.assumptions /\
+        SB.option_prop_sem stpb.chck.assumptions));
+    assert (SB.option_prop_sem stp.chck.obligations <==> (
+        b2t stpg.v /\
+        SB.option_prop_sem stpr.chck.obligations /\
+        SB.option_prop_sem stpg.chck.obligations /\
+        SB.option_prop_sem stpb.chck.obligations));
+    ()
+  | hd :: tl ->
+    let hd' = List.hd rows' in
+    let tl' = List.tl rows' in
+    contract_invariant_holds tl r g b;
+
+    let stp0  = SI.system_step_result t (inputs_with_oracles_contract_definition tl r g b) in
+
+    SXP.invariant_step tl hd r (SB.type_join_fst stp0.s);
+    SXP.invariant_step tl' hd' g (SB.type_join_fst (SB.type_join_snd stp0.s));
+    SXP.invariant_step tl hd b (SB.type_join_snd (SB.type_join_snd stp0.s));
+
+    assert (stp == t.step hd o stp0.s);
+    assert (stpr == (SX.system_of_exp r).step hd (SB.type_join_fst o) (SB.type_join_fst stp0.s));
+    assert (stpb == (SX.system_of_exp b).step hd (SB.type_join_snd (SB.type_join_snd o)) (SB.type_join_snd (SB.type_join_snd stp0.s)));
+    assert (stpg == (SX.system_of_exp g).step (stpb.v, hd) (SB.type_join_fst (SB.type_join_snd o)) (SB.type_join_fst (SB.type_join_snd stp0.s)));
+
+    assert (SB.option_prop_sem stp.chck.assumptions <==> (
+        b2t stpr.v /\
+        SB.option_prop_sem stpr.chck.assumptions /\
+        SB.option_prop_sem stpg.chck.assumptions /\
+        SB.option_prop_sem stpb.chck.assumptions));
+    assert (SB.option_prop_sem stp.chck.obligations <==> (
+        b2t stpg.v /\
+        SB.option_prop_sem stpr.chck.obligations /\
+        SB.option_prop_sem stpg.chck.obligations /\
+        SB.option_prop_sem stpb.chck.obligations));
+    ()
+
+
+
+let rec system_holds_exp_of_contract
+  (#t: table) (#c: context t) (#a: t.ty)
+  (rows: list (row c) { Cons? rows })
+  (r: exp t       c  t.propty { XC.causal r })
+  (g: exp t (a :: c) t.propty { XC.causal g })
+  (b: exp t       c         a { XC.causal b }):
+  Lemma
+    (requires (
+      XK.check_all PM.check_mode_valid r /\
+      XK.check_all PM.check_mode_valid g /\
+      XK.check_all PM.check_mode_valid b /\
+      XB.bigstep_always rows r /\
+      SI.system_holds_all (SX.system_of_contract r g b)
+    ))
+    (ensures (
+      let vs  = XC.lemma_bigsteps_total_vs rows b in
+      let rows'=CR.extend1 vs rows in
+      let ios = inputs_with_oracles_contract_definition rows r g b in
+      let stp = SI.system_step_result (SX.system_of_contract r g b) ios in
+
+      SI.system_assumptions_sofar (SX.system_of_contract r g b) (inputs_with_oracles_contract_definition rows r g b) /\
+
+      check_invariant PM.check_mode_unknown rows r /\
+      check_invariant PM.check_mode_unknown rows' g /\
+      check_invariant PM.check_mode_unknown rows b /\
+      XB.bigstep_always rows' g
+    ))
+  =
+  let vs  = XC.lemma_bigsteps_total_vs rows b in
+  let rows'=CR.extend1 vs rows in
+  let t   = SX.system_of_contract r g b in
+  let ios = inputs_with_oracles_contract_definition rows r g b in
+  let stp = SI.system_step_result t ios in
+
+  let iosr = inputs_with_oracles rows r in
+  let stpr = SI.system_step_result (SX.system_of_exp r) iosr in
+
+  let iosg = inputs_with_oracles rows' g in
+  let stpg = SI.system_step_result (SX.system_of_exp g) iosg in
+
+  let iosb = inputs_with_oracles rows b in
+  let stpb = SI.system_step_result (SX.system_of_exp b) iosb in
+
+  let o = SB.type_join_tup
+    (SXP.step_oracle rows r)
+    (SB.type_join_tup
+      (SXP.step_oracle rows' g)
+      (SXP.step_oracle rows b))
+  in
+  SXCI.check_invariant_of_check_base PM.check_mode_valid rows r;
+  SXCI.check_invariant_of_check_base PM.check_mode_valid rows' g;
+  SXCI.check_invariant_of_check_base PM.check_mode_valid rows b;
+  contract_invariant_holds rows r g b;
+  match rows with
+  | [hd] ->
+    check_init PM.check_mode_unknown r;
+    check_init PM.check_mode_unknown g;
+    check_init PM.check_mode_unknown b;
+
+    SXP.invariant_init r;
+    SXP.invariant_init g;
+    SXP.invariant_init b;
+
+    let hd' = List.hd rows' in
+    assert (rows' == [hd']);
+    assert (check_invariant PM.check_mode_valid [hd'] g);
+    assert (check_invariant PM.check_mode_unknown [] g);
+
+    SXCA.check_step_asm [] hd r (SB.type_join_fst t.init);
+    SXCA.check_step_asm [] hd' g (SB.type_join_fst (SB.type_join_snd t.init));
+    SXCA.check_step_asm [] hd b (SB.type_join_snd (SB.type_join_snd t.init));
+
+    SXCO.check_step_obl [] hd r (SB.type_join_fst t.init);
+    SXCO.check_step_obl [] hd' g (SB.type_join_fst (SB.type_join_snd t.init));
+    SXCO.check_step_obl [] hd b (SB.type_join_snd (SB.type_join_snd t.init));
+    ()
+
+  | hd :: tl ->
+    let hd' = List.hd rows' in
+    let tl' = List.tl rows' in
+    let ios = inputs_with_oracles_contract_definition tl r g b in
+    let stp0 = SI.system_step_result (SX.system_of_contract r g b) ios in
+
+    contract_invariant_holds tl r g b;
+    system_holds_exp_of_contract tl r g b;
+
+    SXCA.check_step_asm tl hd r (SB.type_join_fst stp0.s);
+    SXCA.check_step_asm tl' hd' g (SB.type_join_fst (SB.type_join_snd stp0.s));
+    SXCA.check_step_asm tl hd b (SB.type_join_snd (SB.type_join_snd stp0.s));
+
+    SXCO.check_step_obl tl hd r (SB.type_join_fst stp0.s);
+    SXCO.check_step_obl tl' hd' g (SB.type_join_fst (SB.type_join_snd stp0.s));
+    SXCO.check_step_obl tl hd b (SB.type_join_snd (SB.type_join_snd stp0.s));
+    ()
