src/Pipit.System.Exp.Check.Entailment.fst
@@ -1,0 +1,190 @@
+(* Properties that hold on the translated system hold on the original semantics *)
+module Pipit.System.Exp.Check.Entailment
+
+open Pipit.Prim.Table
+open Pipit.Exp.Base
+open Pipit.System.Exp.Check.Base
+
+module SXCA = Pipit.System.Exp.Check.Assumptions
+module SXCC = Pipit.System.Exp.Check.Contracts
+module SXCI = Pipit.System.Exp.Check.Invariants
+module SXCO = Pipit.System.Exp.Check.Obligations
+
+module CR  = Pipit.Context.Row
+
+module SB  = Pipit.System.Base
+module SX  = Pipit.System.Exp
+module SXP = Pipit.System.Exp.Properties
+module SI  = Pipit.System.Ind
+
+module XB  = Pipit.Exp.Bigstep
+module XC  = Pipit.Exp.Causality
+module XK  = Pipit.Exp.Checked.Base
+
+module PM = Pipit.Prop.Metadata
+
+module List = FStar.List.Tot
+module T    = FStar.Tactics
+
+#push-options "--split_queries always"
+
+let rec entailment
+  (#t: table) (#c: context t) (#a: t.ty)
+  (rows: list (row c))
+  (row1: row c)
+  (e: exp t c a { XC.causal e }):
+  Lemma
+    (requires (
+      XK.check_all PM.check_mode_valid e /\
+      XK.sealed true e /\
+      SI.system_holds_all (SX.system_of_exp e)
+    ))
+    (ensures (
+      let ios = inputs_with_oracles (row1 :: rows) e in
+      let stp = SI.system_step_result (SX.system_of_exp e) ios in
+      XK.check PM.check_mode_unknown (row1 :: rows) e /\
+      check_invariant PM.check_mode_unknown (row1 :: rows) e /\
+      SXP.system_of_exp_invariant (row1 :: rows) e stp.s /\
+      SI.system_assumptions_sofar (SX.system_of_exp e) ios /\
+      SB.option_prop_sem stp.chck.assumptions /\
+      SB.option_prop_sem stp.chck.obligations
+    ))
+  =
+    SXCI.check_invariant_of_check_base PM.check_mode_valid (row1 :: rows) e;
+    let ios  = inputs_with_oracles (row1 :: rows) e in
+    match rows with
+    | [] ->
+      SXP.invariant_init e;
+      check_init PM.check_mode_unknown e;
+      let s0 = (SX.system_of_exp e).init in
+      let stp = eval_step rows row1 e s0 in
+      SXCA.check_step_asm rows row1 e s0;
+      assert (SI.system_assumptions_sofar (SX.system_of_exp e) ios);
+      SXCO.check_step_obl rows row1 e s0;
+      SXCI.check_base_unknown_of_check_invariant (row1 :: rows) e;
+      ()
+    | row1' :: rows' ->
+      entailment rows' row1' e;
+      let ios' = inputs_with_oracles rows e in
+      let stp0 = SI.system_step_result (SX.system_of_exp e) ios' in
+      let stp  = eval_step rows row1 e stp0.s in
+      assert (check_invariant PM.check_mode_valid   (row1 :: rows) e);
+      assert (check_invariant PM.check_mode_unknown          rows  e);
+      SXCA.check_step_asm rows row1 e stp0.s;
+      assert (check_invariant PM.check_mode_valid   (row1 :: rows) e);
+      assert (check_invariant PM.check_mode_unknown          rows  e);
+      assert (SB.option_prop_sem stp.chck.assumptions);
+      assert (SI.system_assumptions_sofar (SX.system_of_exp e) ios);
+      assert (SB.option_prop_sem stp.chck.obligations);
+      SXCO.check_step_obl rows row1 e stp0.s;
+      SXCI.check_base_unknown_of_check_invariant (row1 :: rows) e;
+      ()
+
+
+let entailment_all
+  (#t: table) (#c: context t) (#a: t.ty)
+  (e: exp t c a { XC.causal e }):
+  Lemma
+    (requires (
+      XK.check_all PM.check_mode_valid e /\
+      XK.sealed true e /\
+      SI.system_holds_all (SX.system_of_exp e)
+    ))
+    (ensures (
+      XK.check_all PM.check_mode_unknown e
+    ))
+  =
+    introduce forall (rows: list (row c)). XK.check PM.check_mode_unknown rows e
+    with match rows with
+      | [] -> SXCI.check_base_nil PM.check_mode_unknown e
+      | row1 :: rows ->
+        let stp = entailment rows row1 e in
+        ()
+
+let entailment_contract
+  (#t: table) (#c: context t) (#a: t.ty)
+  (rows: list (row c) { Cons? rows })
+  (r: exp t       c  t.propty { XC.causal r })
+  (g: exp t (a :: c) t.propty { XC.causal g })
+  (b: exp t       c         a { XC.causal b }):
+  Lemma
+    (requires (
+      XK.check_all PM.check_mode_valid r /\
+      XK.check_all PM.check_mode_valid g /\
+      XK.check_all PM.check_mode_valid b /\
+      XK.sealed true r /\
+      XK.sealed true g /\
+      XK.sealed true b /\
+      XB.bigstep_always rows r /\
+      SI.system_holds_all (SX.system_of_contract r g b)
+    ))
+    (ensures (
+      let vs = XC.lemma_bigsteps_total_vs rows b in
+      XK.check PM.check_mode_unknown rows r /\
+      XK.check PM.check_mode_unknown rows b /\
+      XK.check PM.check_mode_unknown (CR.extend1 vs rows) g /\
+      XB.bigstep_always (CR.extend1 vs rows) g
+    ))
+    =
+  let vs  = XC.lemma_bigsteps_total_vs rows b in
+  let rows'=CR.extend1 vs rows in
+  SXCI.check_invariant_of_check_base PM.check_mode_valid rows r;
+  SXCI.check_invariant_of_check_base PM.check_mode_valid (CR.extend1 vs rows) g;
+  SXCI.check_invariant_of_check_base PM.check_mode_valid rows b;
+
+  assert (XB.bigstep_always rows r);
+  assert (SI.system_holds_all (SX.system_of_contract r g b));
+
+  SXCC.system_holds_exp_of_contract rows r g b;
+
+  SXCI.check_base_unknown_of_check_invariant rows r;
+  SXCI.check_base_unknown_of_check_invariant rows' g;
+  SXCI.check_base_unknown_of_check_invariant rows b;
+  ()
+
+let entailment_contract_all
+  (#t: table) (#c: context t) (#a: t.ty)
+  (r: exp t       c  t.propty { XC.causal r })
+  (g: exp t (a :: c) t.propty { XC.causal g })
+  (b: exp t       c         a { XC.causal b }):
+  Lemma
+    (requires (
+      XK.check_all PM.check_mode_valid r /\
+      XK.check_all PM.check_mode_valid g /\
+      XK.check_all PM.check_mode_valid b /\
+      XK.sealed true r /\
+      XK.sealed true g /\
+      XK.sealed true b /\
+      SI.system_holds_all (SX.system_of_contract r g b)
+    ))
+    (ensures (
+      XK.contract_valid r g b
+    ))
+  =
+    introduce
+      forall (rows: list (row c)) (vs: list (t.ty_sem a) { XB.bigsteps_prop rows b vs }).
+      XB.bigstep_always rows r ==>
+      XK.check PM.check_mode_valid rows r ==>
+      XK.check PM.check_mode_valid rows b ==>
+      XK.check PM.check_mode_valid (CR.extend1 vs rows) g ==>
+        (XK.check PM.check_mode_unknown rows b /\
+        XK.check PM.check_mode_unknown (CR.extend1 vs rows) g /\
+        XB.bigstep_always (CR.extend1 vs rows) g)
+    with
+      introduce 
+        XB.bigstep_always rows r ==>
+        (XK.check PM.check_mode_valid rows r ==>
+        XK.check PM.check_mode_valid rows b ==>
+        XK.check PM.check_mode_valid (CR.extend1 vs rows) g ==>
+          (XK.check PM.check_mode_unknown rows b /\
+          XK.check PM.check_mode_unknown (CR.extend1 vs rows) g /\
+          XB.bigstep_always (CR.extend1 vs rows) g))
+      with pf. (
+        (match rows with
+        | [] ->
+          SXCI.check_base_nil PM.check_mode_unknown g;
+          SXCI.check_base_nil PM.check_mode_unknown b
+        | _ -> entailment_contract rows r g b);
+        XB.bigsteps_deterministic_squash rows b vs (XC.lemma_bigsteps_total_vs rows b);
+        ()
+      )
